Refactored registration and vote types

post-cip/formal-crypto/lean/src/Leioscrypto/Vote.lean
@@ -8,32 +8,18 @@ import Leioscrypto.Types
 namespace Leioscrypto
 
 
-
-inductive Vote where
-| PersistentVote : ElectionId → BlockHash → PoolIndex → BLS.Signature → Vote
-| NonpersistentVote : ElectionId → BlockHash → PoolIndex → BLS.Signature → BLS.Signature → Vote
+structure Vote where
+  electionId : ElectionId
+  ebHash : BlockHash
+  poolIndex : PoolIndex
+  sigma_eid : Option BLS.Signature
+  sigma_m : BLS.Signature
 
 namespace Vote
 
-  def electionId : Vote → ElectionId
-  | PersistentVote eid _ _ _ => eid
-  | NonpersistentVote eid _ _ _ _ => eid
-
-  def ebHash : Vote → BlockHash
-  | PersistentVote _ bh _ _ => bh
-  | NonpersistentVote _ bh _ _ _ => bh
-
-  def poolIndex : Vote → PoolIndex
-  | PersistentVote _ _ pi _ => pi
-  | NonpersistentVote _ _ pi _ _ => pi
-
-  def sigma_m : Vote → BLS.Signature
-  | PersistentVote _ _ _ sm => sm
-  | NonpersistentVote _ _ _ sm _ => sm
-
-  def sigma_eid : Vote → Option BLS.Signature
-  | PersistentVote _ _ _ _ => none
-  | NonpersistentVote _ _ _ _ se => some se
+  structure WellFormed (v : Vote) : Prop where
+    wf_sigma_eid : v.sigma_eid.elim True BLS.Signature.WellFormed
+    wf_sigma_m : v.sigma_m.WellFormed
 
   def ValidSignatures (regs : Registry) (ctx : EpochContext) (vote : Vote) : Prop :=
     let poolIndex : Nat := vote.poolIndex
